proving that we can create a shifted list that is not multiple of the previous primes and the next prime

dafny/derivative.dfy
@@ -2,33 +2,63 @@ include "integral.dfy"
 include "list.dfy"
 include "cycle.dfy"
 
-module Derivetive {
+module Derivative {
 
     import Integral
     import List
     import Cycle
 
-    function isDerivetive(list: seq<nat>, initial: nat, listDerivetive: seq<nat>): bool
-        requires |list| == |listDerivetive|;
+    function isDerivative(list: seq<nat>, initial: nat, listDerivative: seq<nat>): bool
+        requires |list| == |listDerivative|;
     {
-        ( forall v: nat :: 0 < v < |list| ==> ( list[v] >= list[v-1] && listDerivetive[v] == list[v] - list[v-1] ) )
+        ( forall v: nat :: 0 < v < |list| ==> ( list[v] >= list[v-1] && listDerivative[v] == list[v] - list[v-1] ) )
         && 
         ( |list| > 0 ==> list[0] > initial )
         && 
-        ( |list| > 0 ==> listDerivetive[0] == list[0] - initial )
+        ( |list| > 0 ==> listDerivative[0] == list[0] - initial )
     }
 
-    lemma isDerivetiveReverseIntegral(list: seq<nat>, listIntegral: seq<nat>, listDerivetive: seq<nat>, initial: nat)
+    method derivative(list: seq<nat>, initial: nat) returns (listDerivative: seq<nat>)
+        requires |list| > 0;
+        requires List.sorted(list);
+        requires list[0] > initial;
+        ensures |list| == |listDerivative|;
+        ensures isDerivative(list, initial, listDerivative);
+    {
+        var distance := |list|;
+        var arr := new nat[distance];
+        var k := 0;
+        arr[0] := list[0] - initial;
+        while (k < |list|)
+            decreases |list| - k;
+            invariant 0 <= k <= |list|;
+            invariant forall v: nat :: 0 < v < k ==> arr[v] == list[v] - list[v-1];
+            invariant arr[0] == list[0] - initial;
+        {
+            if ( k > 0 ) {
+                arr[k] := list[k] - list[k-1];
+            }
+            k := k + 1;
+        }
+        listDerivative := arr[..];
+    }
+
+    /**
+     * listIntegral = integral(list, initial)
+     * listDerivative = derivative(listIntegral, initial)
+     * listDerivative == list
+     */
+    lemma derivativeOfIntegral(list: seq<nat>, listIntegral: seq<nat>, listDerivative: seq<nat>, initial: nat)
         requires |list| == |listIntegral|;
         requires Integral.isIntegral(list, initial, listIntegral);
-        requires |listIntegral| == |listDerivetive|;
-        requires isDerivetive(listIntegral, initial, listDerivetive);
-        ensures list == listDerivetive;
+        requires |listIntegral| == |listDerivative|;
+        requires isDerivative(listIntegral, initial, listDerivative);
+        ensures list == listDerivative;
     {
         if list == [] {
             assert listIntegral == [];
-            assert listDerivetive == [];
-            assert listDerivetive == list;
+            assert listDerivative == [];
+            assert listDerivative == list;
         } else if |list| == 1 {
             var h := list[0];
             assert forall v: nat :: 0 <= v < |list| ==> listIntegral[v] == List.sum(list[0..v+1]) + initial;
@@ -37,13 +67,13 @@ module Derivetive {
             assert listIntegral[0] == List.sum([list[0]]) + initial;
             assert List.sum([list[0]]) == list[0];
             assert listIntegral[0] == list[0] + initial == h + initial;
-            assert listDerivetive[0] == listIntegral[0] - initial;
-            assert listDerivetive[0] == h + initial - initial == h;
-            assert listDerivetive == list;
+            assert listDerivative[0] == listIntegral[0] - initial;
+            assert listDerivative[0] == h + initial - initial == h;
+            assert listDerivative == list;
         } else {
             assert forall v: nat :: 0 <= v < |list| ==> listIntegral[v] == List.sum(list[0..v+1]) + initial;
             forall k | 0 < k < |listIntegral|
-                ensures listDerivetive[k] == list[k];
+                ensures listDerivative[k] == list[k];
             {
                 assert listIntegral[k] >= listIntegral[k-1];
                 assert listIntegral[k] == List.sum(list[0..k+1]) + initial;
@@ -53,13 +83,96 @@ module Derivetive {
                 assert List.sum(list[0..k+1]) == List.sum(list[0..k] + [list[k]]);
                 assert List.sum(list[0..k+1]) == List.sum(list[0..k]) + List.sum([list[k]]);
                 assert List.sum(list[0..k+1]) == List.sum(list[0..k]) + list[k];
-                assert listDerivetive[k] == listIntegral[k] - listIntegral[k-1];
-                assert listDerivetive[k] == (List.sum(list[0..k+1]) + initial) - (List.sum(list[0..k]) + initial);
-                assert listDerivetive[k] == List.sum(list[0..k+1]) + initial - List.sum(list[0..k]) - initial;
-                assert listDerivetive[k] == List.sum(list[0..k]) + list[k] + initial - List.sum(list[0..k]) - initial;
-                assert listDerivetive[k] == list[k] + List.sum(list[0..k]) - List.sum(list[0..k]) + initial - initial;
-                assert listDerivetive[k] == list[k];
+                assert listDerivative[k] == listIntegral[k] - listIntegral[k-1];
+                assert listDerivative[k] == (List.sum(list[0..k+1]) + initial) - (List.sum(list[0..k]) + initial);
+                assert listDerivative[k] == List.sum(list[0..k+1]) + initial - List.sum(list[0..k]) - initial;
+                assert listDerivative[k] == List.sum(list[0..k]) + list[k] + initial - List.sum(list[0..k]) - initial;
+                assert listDerivative[k] == list[k] + List.sum(list[0..k]) - List.sum(list[0..k]) + initial - initial;
+                assert listDerivative[k] == list[k];
             }
         }
+    }
+
+    /**
+     * listDerivative = derivative(list, initial)
+     * listIntegral = integral(listDerivative, initial)
+     * listDerivative == list
+     */
+    lemma integralOfDerivative(list: seq<nat>, listDerivative: seq<nat>, listIntegral: seq<nat>, initial: nat)
+        requires |list| == |listDerivative|;
+        requires |listIntegral| == |list|;
+        requires isDerivative(list, initial, listDerivative);
+        requires Integral.isIntegral(listDerivative, initial, listIntegral);
+        requires |listIntegral| == |listDerivative|;
+        ensures list == listIntegral;
+    {
+        if list == [] {
+            assert listIntegral == [];
+            assert listDerivative == [];
+            assert listDerivative == list;
+        } else if |list| == 1 {
+            var h := list[0];
+            assert forall v: nat :: 0 <= v < |listDerivative| ==> listIntegral[v] == List.sum(listDerivative[0..v+1]) + initial;
+            assert listIntegral[0] == List.sum(listDerivative[0..1]) + initial;
+            assert listDerivative[0..1] == [listDerivative[0]];
+            assert listIntegral[0] == List.sum([listDerivative[0]]) + initial;
+            assert List.sum([listDerivative[0]]) == listDerivative[0];
+            assert listIntegral[0] == listDerivative[0] + initial;
+            assert listDerivative[0] == list[0] - initial;
+            assert listIntegral[0] == list[0] - initial + initial;
+            assert listIntegral[0] == list[0];
+            assert listIntegral == list;
+        } else {
+            assert forall v: nat :: 0 <= v < |list| ==> listIntegral[v] == List.sum(listDerivative[0..v+1]) + initial;
+            var k := 0;
+            while (k < |listIntegral|)
+                decreases |listIntegral| - k;
+                invariant 0 <= k <= |listIntegral|;
+                invariant forall v: nat :: 0 <= v < k ==> listIntegral[v] == list[v];
+            {
+                if ( k == 0 ) {
+                    assert listDerivative[0] == list[0] - initial;
+                    assert listIntegral[0] == List.sum(listDerivative[0..1]) + initial;
+                    assert listDerivative[0..1] == [listDerivative[0]];
+                    assert listIntegral[0] == List.sum([listDerivative[0]]) + initial;
+                    assert List.sum([listDerivative[0]]) == listDerivative[0];
+                    assert listIntegral[0] == listDerivative[0] + initial;
+                    assert listIntegral[0] == list[0] - initial + initial;
+                    assert listIntegral[0] == list[0];
+                } else {
+                    assert listIntegral[k] == List.sum(listDerivative[..k+1]) + initial;
+                    assert listDerivative[..k+1] == listDerivative[..k]+[listDerivative[k]];
+                    assert listIntegral[k] == List.sum(listDerivative[..k]+[listDerivative[k]]) + initial;
+                    List.distributiveSum(listDerivative[..k],[listDerivative[k]]);
+                    assert listIntegral[k] == List.sum(listDerivative[..k]) + List.sum([listDerivative[k]]) + initial;
+                    assert listIntegral[k] == List.sum(listDerivative[..k]) + initial + List.sum([listDerivative[k]]);
+                    assert listIntegral[k-1] == List.sum(listDerivative[..k]) + initial;
+                    assert listIntegral[k] == listIntegral[k-1] + List.sum([listDerivative[k]]);
+                    assert List.sum([listDerivative[k]]) == listDerivative[k];
+                    assert listIntegral[k] == listIntegral[k-1] + listDerivative[k];
+                    assert listIntegral[k-1] == list[k-1];
+                    assert listIntegral[k] == list[k-1] + list[k] - list[k-1];
+                    assert listIntegral[k] == list[k] + list[k-1] - list[k-1];
+                    assert listIntegral[k] == list[k];
+                }
+                k := k + 1;
+            }
+        }
+    }
+
+    lemma sumOfDerivativeEqualsLastElement(listIntegral: seq<nat>, listDerivative: seq<nat>, initial: nat)
+        requires |listIntegral| > 0;
+        requires |listDerivative| == |listIntegral|;
+        requires Integral.isIntegral(listDerivative, initial, listIntegral);
+        requires |listIntegral| == |listDerivative|;
+        ensures List.last(listIntegral) == List.sum(listDerivative) + initial;
+    {
+        assert |listIntegral| == |listDerivative|;
+        assert listIntegral[ |listIntegral| - 1 ] == List.sum(listDerivative[..|listIntegral|]) + initial;
+        assert listIntegral[ |listIntegral| - 1 ] == List.sum(listDerivative[..|listDerivative|]) + initial;
+        assert listDerivative[..|listDerivative|] == listDerivative;
+        assert listIntegral[ |listIntegral| - 1 ] == List.sum(listDerivative) + initial;
+        assert List.last(listIntegral) == listIntegral[ |listIntegral| - 1 ];
+        assert List.last(listIntegral) == List.sum(listDerivative) + initial;
     }
 }
